cedar-lean/Cedar/Spec/Value.lean
@@ -139,7 +139,7 @@ instance : LawfulBEq Attr where
     assumption
 
 
-deriving instance Repr, DecidableEq, BEq, LT  for Attr
+deriving instance Repr, DecidableEq, BEq, LT for Attr
 deriving instance Repr, DecidableEq, BEq for Except
 deriving instance Repr, DecidableEq for Error
 deriving instance Repr, DecidableEq, Inhabited, Lean.ToJson for Name
@@ -147,6 +147,8 @@ deriving instance Repr, DecidableEq, Inhabited for EntityType
 deriving instance Repr, DecidableEq, Inhabited for EntityUID
 deriving instance Repr, DecidableEq, Inhabited for Prim
 deriving instance Repr, Inhabited for Value
+
+
 
 mutual
 
@@ -200,6 +202,9 @@ instance : LT Name where
 
 instance Name.decLt (a b : Name) : Decidable (a < b) :=
   if h : Name.lt a b then isTrue h else isFalse h
+
+instance Attr.decLt (a b : Attr) : Decidable (a < b) :=
+  if h : a < b then isTrue h else isFalse h
 
 def EntityUID.lt (a b : EntityUID) : Bool :=
   (a.ty < b.ty) ∨ (a.ty = b.ty ∧ a.eid < b.eid)
